examples/spinlock/SpinLockAll.v
@@ -200,3 +200,175 @@ Module SpinLockAll.
     { exists x; des; eauto. }
   Qed.
 End SpinLockAll.
+
+Module SpinLockAllFail.
+  Import inv_instances.
+  Local Instance Γ : HRA := ##[invΓ; memΓ; SchAΓ; SpinLockΓ; SpinLockMainAΓ].
+  Local Instance Σ : GRA := ##[invΣ; SchAΣ; Γ].
+
+  (* building the target module *)
+  Local Definition csl : string → bool := λ _, false.
+  Local Definition genv : GEnv.t := GEnv.unit.
+  Local Definition mod_tgt : HMod.t := SpinLockMainI.t ★ MemI.t csl genv ★ SchI.t ★ SpinLockI.t.
+
+  (* building the source module *)
+  Local Definition u : univ_id := 1.
+
+  Local Definition spc_user_s : string → option fspec :=
+    to_spc (SpinLockMainAS.spc u ++ MemA.Spc ++ SpinLockAS.spc u).
+
+  Local Definition smod_src : SMod.t :=
+    SpinLockMainA.Mod u ☆ MemA.Mod ☆ SchA.Mod u spc_user_s ☆ SpinLockA.Mod u.
+  Local Definition spc_s : string → option fspec :=
+    spc_from smod_src.
+  Local Definition mod_src : HMod.t := SMod.to_hmod (wsim_ginv u ⊤) spc_s smod_src.
+  Local Definition init_cond : iProp Σ := (MemA.InitCond csl genv ∗ SchA.InitCond)%I.
+
+  (* source module after cancellation *)
+  Local Definition smod_cancel : HMod.t := SModCancel.to_hmod smod_src.
+
+  (* Refinement between smod_cancel and smod_src *)
+  Local Definition main_fsp : fspec := SpinLockMainAS.main_spec u.
+  Lemma cancel_src :
+    refines (smod_cancel, init_cond ∗ main_fsp.(precond) tt tt↑ tt↑)%I
+            (mod_src,     init_cond).
+  Proof. eapply cancellation; try by econs. i. unfold_pre_post. iIntros "[_ [-> ->]]". done. Qed.
+
+  (* Refinement between smod_src and mod_tgt *)
+  Lemma src_tgt : refines (mod_src, init_cond) (mod_tgt, emp%I).
+  Proof.
+    apply ctxr_refines.
+    rewrite /mod_src /smod_src /mod_tgt /init_cond ?add_interp_comm.
+    etrans.
+    { do 2 eapply ctxr_frameL. eapply ctxr_comm. }
+    do 2 rewrite -hmod_add_assoc.
+    etrans.
+    { eapply ctxr_frameR.
+      replace (SMod.to_hmod _ _ (SpinLockMainA.Mod _)) with (SpinLockMainA.t u spc_s); cycle 1.
+      { unfold_hmod; ss. }
+      replace (SMod.to_hmod _ _ (MemA.Mod)) with (MemA.t u spc_s); cycle 1.
+      { unfold_hmod; ss. }
+      replace (SMod.to_hmod _ _ (SpinLockA.Mod _)) with (SpinLockA.t u spc_s); cycle 1.
+      { unfold_hmod; ss. }
+      rewrite hmod_add_assoc -hmod_addc_empty_l.
+      etrans; first eapply ctxr_cond_frameR.
+      { eapply SpinLockMainIA.wctxr; eauto.
+        { instantiate (1:=spc_user_s).
+          rewrite /spc_user_s /SchAS.spc /spc_s /smod_src; unseal CRIS. split; first prove_nodup.
+          ii. ss; des_ifs; rewrite ->eq_rel_dec_correct in *; des_ifs.
+        }
+        { rewrite /spc_user_s /SchAS.spc /spc_s /smod_src; unseal CRIS. split; first prove_nodup.
+          ii. ss; des_ifs; rewrite ->eq_rel_dec_correct in *; des_ifs.
+        }
+        { rewrite /spc_user_s /MemA.Spc /spc_s /smod_src; unseal CRIS. split; first prove_nodup.
+          ii. ss; des_ifs; rewrite ->eq_rel_dec_correct in *; des_ifs.
+        }
+      }
+      rewrite hmod_addc_empty_l. refl.
+    }
+    rewrite hmod_add_assoc. eapply ctxr_frameL.
+    etrans.
+    { eapply ctxr_frameR. rewrite -hmod_addc_empty_l. eapply ctxr_cond_frameR.
+      etrans; first eapply ctxr_comm.
+      eapply SpinLockIA.wctxr.
+      { rewrite /spc_user_s /SchAS.spc /spc_s /smod_src; unseal CRIS. split; first prove_nodup.
+        ii. ss; des_ifs; rewrite ->eq_rel_dec_correct in *; des_ifs.
+      }
+      { rewrite /spc_user_s /spc_s /smod_src /MemA.Spc; unseal CRIS. split; first prove_nodup.
+        ii. ss; des_ifs; rewrite ->eq_rel_dec_correct in *; des_ifs.
+      }
+    }
+    rewrite hmod_add_assoc.
+    etrans; first eapply ctxr_comm. rewrite -hmod_add_assoc. eapply ctxr_frameR.
+    etrans.
+    { rewrite hmod_addc_empty_l. eapply ctxr_frameR, ctxr_cond_frameR. eapply MemIA.wctxr.
+      rewrite /MemA.Spc; unseal CRIS.
+      split; first prove_nodup. ii; ss; des_ifs; rewrite ->eq_rel_dec_correct in *; des_ifs.
+    }
+    eapply ctxr_frameL.
+    etrans.
+    { replace (SMod.to_hmod _ _ (SchA.Mod _ _)) with (SchA.t u spc_s spc_user_s); cycle 1.
+      { unfold_hmod; ss. }
+      rewrite hmod_addc_empty_l.
+      eapply SchIA.wctxr.
+      { rewrite /spc_user_s /SchAS.spc /spc_s /smod_src; unseal CRIS. split; first prove_nodup.
+        ii. ss; des_ifs; rewrite ->eq_rel_dec_correct in *; des_ifs.
+      }
+      { rewrite /spc_user_s /SchAS.spc /spc_s /smod_src /MemA.Spc; unseal CRIS.
+        ii. ss; des_ifs; rewrite ->eq_rel_dec_correct in *; des_ifs.
+      }
+    }
+    refl.
+  Qed.
+
+  Lemma cancel_tgt :
+    refines (smod_cancel, (init_cond ∗ (main_fsp).(precond) tt tt↑ tt↑)%I)
+            (mod_tgt, emp%I).
+  Proof.
+    etrans.
+    { eapply cancel_src. }
+    { eapply src_tgt. }
+  Qed.
+
+  Import rListNotations.
+  Local Definition initial_resource_list : res_list :=
+    [ownIRA_resource u; ownERA_resource u; ownDRA_resource u; SchAS.tidRA_resource; SchAS.threadsRA_resource]%res_list.
+  Local Definition initial_resource : Σ := 
+    (op_res_list initial_resource_list) ⋅ initial_resource_own_admin.
+
+  Ltac solve_eq_index :=
+    match goal with
+    | H : eq_index ?r ?r2 |- _ => revert H; autounfold with GRA_index; intros H; rewrite /eq_index in H
+    end; des_ifs;
+    match goal with
+    | H1 : @eq (inG _ _) ?a _, H2 : @eq (inG _ _) ?b _ |- _ =>
+        let H := fresh "H" in assert (H : inG_id a = inG_id b) by rewrite H1 H2 //=;
+        repeat match goal with
+        | H : inG_id ?a = inG_id ?b |- _ => rewrite /a /b in H
+        end;
+        (* rewrite /a /b in H *)
+        revert H; autounfold with GRA_index; inv_instances.solve_in_subG_goal;
+        rewrite /eq_rec_r /eq_rec /= /subG_inG -!eq_rect_eq //=
+    end.
+  Ltac solve_nin_aux :=
+    match goal with
+    | H : r_In ?RES (r_cons ?RA ?RES' ?tl) |- _ => destruct H as [EQ | IN]; [solve_eq_index| solve_nin_aux]
+    | H : r_In ?RES (r_nil) |- _ => inv H
+    end.
+  Ltac solve_nin := ii; solve_nin_aux.
+  Ltac dfs_solve :=
+    match goal with
+    | |- r_NoDup (r_cons ?RA ?RES ?tl) => econs; [solve_nin|dfs_solve]
+    | |- r_NoDup (r_nil) => econs
+    end.
+  Hint Unfold sProp.in_subG_obligation_1 in_subG subG_invΣ subG_invΓ invG_subG invΓ invΣ invG_Σ invG_Γ invG_D invG_E invG_I SchAΣ : GRA_index.
+  Hint Unfold ownIRA_resource ownERA_resource ownDRA_resource SchAS.tidRA_resource SchAS.threadsRA_resource : GRA_index.
+
+  Theorem behavioral_refinement :
+    ∃ target_resource, refines_mod
+      (HMod.to_mod smod_cancel initial_resource)
+      (HMod.to_mod mod_tgt target_resource).
+  Proof.
+    move: (cancel_tgt)=>H; rewrite /refines in H; ss.
+    destruct (H initial_resource).
+    { apply op_res_list_valid. rewrite /initial_resource_list. dfs_solve. }
+    { iIntros "H". iPoseProof (big_bang with "H") as "[O H]".
+      iPoseProof (ownI_initial_gen with "[H]") as "[U W]".
+      { rewrite /initial_resource_list; s. des_ifs. rename inG_id into i.
+        assert (H' : inG_id invariants.ownIRA_resource_obligation_1 = i).
+        { rewrite Heq; ss. }
+        revert H'. rewrite /invariants.ownIRA_resource_obligation_1 /invG_I. autounfold with GRA_index.
+        rewrite inG_id_subG_inG subG_app_l_inG_id /eq_rec_r /eq_rec -eq_rect_eq.
+        intros H'; ss.
+        iDestruct "H" as "[H1 [H2 [H3 _]]]"; iFrame.
+        eapply eq_ind; first iExact "H1".
+        f_equiv. ss.
+      }
+      iFrame. unfold_pre_post. iSplitL.
+      { rewrite /init_cond. admit. }
+      admit.
+    }
+    { econs; ss; prove_nodup. }
+    { exists x; des; eauto. }
+     
+  Admitted.
